---
title: random2
layout: yo
---

Indicies
	$a^m \times a^n = a^{m+n}$
	$\frac{a^m}{a^n} = a^{m-n}$
	$(a^m)^n = a^{mn}$
	$(ab)^n = a^n b^n$
	$\left(\frac{a}{b}\right)^n = \frac{a^n}{b^n}$
	$a^0 = 1 \quad ( a \neq 0)$
	$a^{-n} = \frac{1}{a^n}$
	$a^{\frac{m}{n}} = \sqrt[n]{a^m} = (\sqrt[n]{a})^m$

Surds
    $\sqrt[n]{ab} = \sqrt[n]{a} \times \sqrt[n]{b}$
    $\sqrt[n]{\frac{a}{b}} = \frac{\sqrt[n]{a}}{\sqrt[n]{b}}$
    $\sqrt{a^2 b} = a\sqrt{b}$
    $p\sqrt[n]{a} + q\sqrt[n]{a} = (p+q)\sqrt[n]{a}$
    $\frac{1}{\sqrt{a}} = \frac{1}{\sqrt{a}} \times \frac{\sqrt{a}}{\sqrt{a}} = \frac{\sqrt{a}}{a}$
    $\frac{1}{a + \sqrt{b}} = \frac{1}{a + \sqrt{b}} \times \frac{a - \sqrt{b}}{a - \sqrt{b}} = \frac{a - \sqrt{b}}{a^2 - b}$

Logarithms 



Let $b$, $x$, and $y$ be positive real numbers, where $b \neq 1$.
The base of the logarithm is denoted by $b$.

    $\log_b x = y \iff b^y = x$
    (This means "the exponent to which $b$ must be raised to get $x$ is $y$")

    $\log_b 1 = 0$
    (Since $b^0 = 1$)

    $\log_b b = 1$
    (Since $b^1 = b$)

    $\log_b (xy) = \log_b x + \log_b y$

    $\log_b \left(\frac{x}{y}\right) = \log_b x - \log_b y$

    $\log_b (x^p) = p \log_b x$
	(where $p$ is any real number)

    $\log_b x = \frac{\log_c x}{\log_c b}$
	(where $c$ is any other valid base, often $e$ for $\ln$ or $10$ for $\log_{10}$)

    $b^{\log_b x} = x$
    $\log_b (b^x) = x$

	$\log x = \log_{10} x$
	$\ln x = \log_e x$



---



$\displaystyle m=\frac{rise}{run}=\frac{y_2-y_1}{x_2-x_1}=\frac{change\space in\space y}{change\space in\space x}=\frac{\Delta y}{\Delta x}=\frac{dy}{dx}=f'(x)=y'= \lim_{h \to 0} \frac{f(x+h) - f(x)}{h}$

Slope-Intercept Form
$y=mx+b$
$y=mx+c$

Standard form
$Ax+By=C$

Point-Slope form
$y-y_1=m(x-x_1)$

Distance
$d= \sqrt{(x_2-x_1)^2+(y_2-y_1)^2}$

Midpoint
$m=(\frac{x_1+x_2}{2},\frac{y_1+y_2}{2})$

Parallel 
$m_1=m_2$

Perpendicular 
$m_1\times m_2=-1$
$m_2=-\frac{1}{m_1}$

$d_\perp = \frac{|Ax_1 + By_1 + C|}{\sqrt{A^2 + B^2}}$

Circle
$(x-a)^2+(y-b)^2=r^2$
$(a,b) =$ Centre point of the circle
$r =$ Radius

## Calculus?

$f'(x)=y'$

First Principles: $\displaystyle f'(x) = \lim_{h \to 0} \frac{f(x+h) - f(x)}{h}$ 
Power rule: $f'(x)=nx^{n-1}$

Product rule: $f'(x)=uv'+vu'$
Quotient rule: $f'(x)=\frac{vu'-uv'}{v^2}$ (top is always $u$ and bottom is always $v$)

